commit

Snoclist.v
@@ -25,28 +25,37 @@ Notation "[ x ; y ; .. ; z ]" := (snoc (snoc .. (snoc nil x) .. y) z)
 End SnoclistNotations.
 Import SnoclistNotations.
 
-Theorem snoclist_comm {A : Type} {n m : nat} : snoclist A (m + n) -> snoclist A (n + m).
-Proof. rewrite Nat.add_comm. intro h. apply h. Qed.
+Definition snoclist_npz {A : Type} {n : nat} (l : snoclist A n) : snoclist A (n + 0) :=
+eq_rect n (snoclist A) l (n + 0) (eq_sym (Nat.add_0_r n)).
 
-Theorem snoclist_asso_1 {A : Type} {n m : nat} : snoclist A (S m + n) -> snoclist A (m + S n).
-Proof. rewrite Nat.add_succ_comm. intro h. apply h. Qed.
+Definition snoclist_asso_1 {A : Type} {m n : nat} (l : snoclist A (S m + n)) : snoclist A (m + S n) :=
+eq_rect (S m + n) (snoclist A) l (m + S n) (Nat.add_succ_comm m n).
+
+Fixpoint app {A : Type} {m n : nat} (l : snoclist A m) (r : snoclist A n) :=
+match r with
+| [] => snoclist_npz l
+| r' :: a => snoclist_asso_1 ((app l r') :: a)
+end.
 
 (*
-Theorem snoclist_nil {A : Type} {m : nat} : snoclist A (m + 0) -> snoclist A m.
-Proof. rewrite Nat.add_comm. intro h. apply h. Qed.
+with snoclist_npz {A : Type} {n : nat} (l : snoclist A n) : snoclist A (n + 0) :=
+match l with
+| [] => []
+| l' :: a => snoclist_npz l' :: a
+end
 
-Fixpoint app {A : Type} {n m : nat} (l : snoclist A n) (r : snoclist A m) : snoclist A (n + m) :=
-match r in (snoclist _ m) return (snoclist _ (m + n) -> snoclist _ (n + m)) -> snoclist _ (n + m) with
-| nil => fun H => H l
-| r' :: a => fun _ => (app l r') :: a
-end snoclist_nil.
+with snoclist_asso_1 {A : Type} {m n : nat} (l : snoclist A (S m + n)) : snoclist A (m + S n) :=
+match l in (snoclist _ len) return (len <> 0) -> snoclist _ (m + S n) with
+| [] => fun H => match H eq_refl with end
+| l' :: a => fun _ => 
+  match l' with
+  | [] => aux l
+  | _ => (snoclist_asso_1 l') :: a
+  end
+end Nat.neq_succ_0
+
+with aux {A : Type} (l : snoclist A 1) : snoclist A (0 + 1) := l.
 *)
-
-Fixpoint app {A : Type} {n m : nat} (l : snoclist A n) (r : snoclist A m) : snoclist A (n + m) :=
-match r in (snoclist _ m) return (snoclist _ (m + n) -> snoclist _ (n + m)) -> snoclist _ (n + m) with
-| nil => fun H => H l
-| r' :: a => fun H => H ( snoclist_comm (app l r') :: a)
-end snoclist_comm.
 
 Infix "++" := app (right associativity, at level 60) : snoclist_scope.
 
@@ -60,36 +69,101 @@ intros A l.
 dependent destruction l. reflexivity.
 Qed.
 
-Lemma comm_nil : forall (A : Type), snoclist_comm [] (A := A) (m := 0) (n := 0) = [].
+Lemma nil_npz : forall {A : Type},
+  snoclist_npz [] (A := A) = [].
 Proof.
-intro A. rewrite zero_len with (l := snoclist_comm [] (m := 0) (n := 0)).
+intro A.
+rewrite zero_len with (l := snoclist_npz []).
 reflexivity.
 Qed.
 
-Axiom comm_appnil : forall (A : Type) (n : nat) (l : snoclist A n) (a : A),
-  snoclist_comm (l :: a) (m := 0) (n := S n) = snoclist_comm l (m := 0) (n := n) :: a.
+Axiom snoc_npz : forall {A : Type} (n : nat) (l : snoclist A n) (a : A),
+  snoclist_npz (l :: a) = (snoclist_npz l) :: a.
 
-Axiom comm_nilapp : forall (A : Type) (n : nat) (l : snoclist A n) (a : A),
-  snoclist_comm (snoclist_comm ([] ++ l) :: a) (m := S n) (n := 0) = l :: a.
+Lemma map_npz : forall {A : Type} (n : nat) (l : snoclist A n)
+  (P : forall {n : nat}, snoclist A n -> snoclist A n)
+  (f : A -> A),
+  (forall {n : nat} (l : snoclist A n) (a : A), P (l :: a) = P l :: f a) ->
+  P (snoclist_npz l) = snoclist_npz (P l).
+Proof.
+intros A n l P f h.
+induction l.
+- simpl.
+  rewrite zero_len with (l := snoclist_npz []).
+  rewrite zero_len with (l := snoclist_npz (P 0 [])).
+  rewrite zero_len with (l := P 0 []).
+  reflexivity.
+- simpl.
+  rewrite snoc_npz.
+  rewrite ? h.
+  rewrite snoc_npz.
+  rewrite IHl.
+  reflexivity.
+Qed.
 
-Axiom comm_consapp_asso : forall (A : Type) (m n : nat) (l : snoclist A m) (r : snoclist A n) (a : A),
-  snoclist_comm (snoclist_comm (l ++ r) (m := m) (n := n) :: a) (m := S n) (n := m) =
-  snoclist_asso_1 ((l ++ r) :: a).
+(* TODO *)
+Axiom map_asso : forall {A : Type} (m n : nat) (l : snoclist A (S m + n))
+  (P : forall {n : nat}, snoclist A n -> snoclist A n)
+  (f : A -> A),
+  (forall {n : nat} (l : snoclist A n) (a : A), P (l :: a) = P l :: f a) ->
+  P (snoclist_asso_1 l) = snoclist_asso_1 (P l).
 
-Axiom comm_consapp_asso' : forall (A : Type) (m n : nat) (l : snoclist A m) (r : snoclist A n) (a b : A),
-  snoclist_comm (snoclist_comm ((l :: a) ++ r) (m := S m) (n := n) :: b) (m := S n) (n := S m) =
-  snoclist_asso_1 ((l :: a) ++ r) :: b.
-
-Axiom asso_eq : forall {A : Type} {m n : nat} (l1 l2 : snoclist A (S m + n)),
-  snoclist_asso_1 l1 (m := m) (n := n) = snoclist_asso_1 l2 (m := m) (n := n) -> l1 = l2.
+(*
+Axiom P_npz : forall {A : Type} (n : nat) (l : snoclist A n)
+  (P : forall {n : nat}, snoclist A n -> snoclist A n),
+  P (snoclist_npz l) = snoclist_npz (P l).
 
 Axiom P_asso : forall {A : Type} (m n : nat) (l : snoclist A (S m + n))
   (P : forall {n : nat}, snoclist A n -> snoclist A n),
   P (snoclist_asso_1 l) = snoclist_asso_1 (P l).
+*)
 
-Axiom P_comm : forall {A : Type} (m n : nat) (l : snoclist A (m + n))
-  (P : forall {n : nat}, snoclist A n -> snoclist A n),
-  P (snoclist_comm l) = snoclist_comm (P l).
+Axiom sing_asso : forall {A : Type} (a : A),
+  snoclist_asso_1 ([a]) (m := 0) (n := 0) = [a].
+
+Axiom snoc_asso : forall {A : Type} (m n : nat) (l : snoclist A (S m + n)) (a : A),
+  snoclist_asso_1 (l :: a) (m := (S m)) (n := n) =
+  snoclist_asso_1 l :: a.
+
+(*
+Lemma map_asso : forall {A : Type} (m n : nat) (l : snoclist A (m + n)) (a : A)
+  (P : forall {n : nat}, snoclist A n -> snoclist A n)
+  (f : A -> A),
+  (forall {n : nat} (l : snoclist A n) (a : A), P (l :: a) = P l :: f a) ->
+  P (snoclist_asso_1 (l :: a)) = snoclist_asso_1 (P (l :: a)).
+Proof.
+intros A m n l a P f h.
+dependent induction l.
+- rewrite h.
+  dependent destruction n.
+  dependent destruction m.
+  + simpl.
+    simpl in l0.
+    rewrite zero_len with (l := l0).
+    rewrite zero_len with (l := P 0 []).
+    rewrite ? sing_asso.
+    rewrite h.
+    rewrite zero_len with (l := P 0 []).
+    reflexivity.
+  + simpl in x0.
+    apply eq_sym in x0.
+    apply (Nat.neq_succ_0 (m + 0)) in x0.
+    contradiction.
+  + rewrite <- Nat.add_succ_comm in x0.
+    simpl in x0.
+    apply eq_sym in x0.
+    apply (Nat.neq_succ_0 (m + n)) in x0.
+    contradiction.
+- rewrite h.
+  dependent destruction n.
+  dependent destruction m.
+  + simpl in x0.
+    apply (Nat.neq_succ_0 (n0)) in x0.
+    contradiction.
+  + rewrite snoc_asso.
+*)
+
+
 
 End Facts.
 
@@ -109,10 +183,40 @@ apply inj_pair2_eq_dec in H0.
 Qed.
 
 (*
-Redefine app
 Prove some of those axioms maybe
 Redefine sat_xi (subst ty1 = subst ty2)
 x = y -> P x -> P y?
 *)
 
+(*
+Fixpoint app {A : Type} {n m : nat} (l : snoclist A n) (r : snoclist A m) : snoclist A (n + m) :=
+match r in (snoclist _ m) return (snoclist _ (m + n) -> snoclist _ (n + m)) -> snoclist _ (n + m) with
+| nil => fun H => H l
+| r' :: a => fun H => H ( snoclist_comm (app l r') :: a)
+end snoclist_comm.
+*)
 
+(*
+Lemma app_aux {A : Type} {m n : nat} :
+match n with
+| 0 => snoclist A m -> snoclist A (m + 0)
+| S n => snoclist A (S m + n) -> snoclist A (m + S n)
+end.
+Proof.
+destruct n.
+apply snoclist_npz.
+apply snoclist_asso_1.
+Qed.
+
+Fixpoint app {A : Type} {m n : nat} (l : snoclist A m) (r : snoclist A n) : snoclist A (m + n) :=
+match r as r in (snoclist _ n) return
+ (match n return Type with
+  | 0 => (snoclist _ m -> snoclist _ (m + 0))
+  | S n => (snoclist A (S m + n) -> snoclist A (m + S n))
+  end) ->
+  snoclist A (m + n)
+with
+| [] => fun H => H l
+| r' :: a => fun H => H ((app l r') :: a)
+end app_aux.
+*)
