Workbench.v
@@ -13,6 +13,281 @@ Require Import Coq.Sorting.Permutation.
 Require Import Arith.
 Require List.
 
+Inductive sat_xi : s_rules -> constraints -> Prop :=
+| sat_nil sigma : sat_xi sigma List.nil
+| sat_cons sigma ty1 ty2 const :
+  sat_xi sigma const ->
+  subst_ty sigma ty1 = subst_ty sigma ty2 ->
+  sat_xi sigma (List.cons (ty1, ty2) const).
+
+Lemma app_sat_xi : forall (sigma : s_rules) (const1 const2 : constraints),
+  sat_xi sigma const1 -> sat_xi sigma const2 -> sat_xi sigma (const1 ++ const2)%list.
+Proof.
+intros sigma const1 const2 h1 h2.
+induction const1.
+- simpl. apply h2.
+- simpl.
+  dependent destruction h1.
+  apply sat_cons.
+  apply IHconst1.
+  apply h1.
+  apply H.
+Qed.
+
+Lemma perm_sat_xi : forall (sigma : s_rules) (const1 const2 : constraints),
+  Permutation const1 const2 -> sat_xi sigma const1 -> sat_xi sigma const2.
+Proof.
+intros sigma const1 const2 hp.
+induction hp.
+- intro hs. apply hs.
+- case x. intros ty1 ty2.
+  intro hs. dependent destruction hs.
+  apply sat_cons.
+  + apply IHhp. apply hs.
+  + apply H.
+- case x. intros ty1 ty2.
+  case y. intros ty1' ty2'.
+  intro hs.
+  dependent destruction hs.
+  dependent destruction hs.
+  apply sat_cons. apply sat_cons.
+  + apply hs.
+  + apply H0.
+  + apply H.
+- intro hl.
+  apply IHhp2.
+  apply IHhp1.
+  apply hl.
+Qed.
+
+Lemma extra_sat_xi : forall (sigma : s_rules) (x : type_eq) (const : constraints),
+  sat_xi sigma (x :: const)%list -> sat_xi sigma const.
+Proof. intros. dependent destruction H. apply H. Qed.
+
+Lemma appleft_sat_xi : forall (sigma : s_rules) (const1 const2 : constraints),
+  sat_xi sigma (List.app const1 const2) -> sat_xi sigma const1.
+Proof.
+induction const2.
+- rewrite List.app_nil_r. intro h. apply h.
+- intro h. apply IHconst2.
+  assert (Permutation (const1 ++ a :: const2)%list (a :: (const1 ++ const2))%list).
+  apply (Permutation_sym (Permutation_cons_app
+    (l := (const1 ++ const2)) const1 const2 a
+    (Permutation_refl (const1 ++ const2)))).
+  assert (sat_xi sigma (a :: const1 ++ const2)%list).
+  apply perm_sat_xi with (const1 := (const1 ++ a :: const2)%list).
+  apply H. apply h.
+  apply extra_sat_xi with (x := a).
+  apply H0.
+Qed.
+
+Lemma appright_sat_xi : forall (sigma : s_rules) (const1 const2 : constraints),
+  sat_xi sigma (List.app const1 const2) -> sat_xi sigma const2.
+Proof.
+induction const1.
+- simpl. intros const2 h. apply h.
+- intros const2 h. apply IHconst1.
+  simpl in h.
+  apply extra_sat_xi with (x := a).
+  apply h.
+Qed.
+
+Theorem bidir_typed_syn :
+  forall {n : nat} (gamma : context n) (st : sterm n) (ty : type) (const : constraints) (sigma : s_rules),
+  is_bidir_syn gamma st ty const ->
+  sat_xi sigma const ->
+  is_typed (subst_ctx sigma gamma) (strip_syn st) (subst_ty sigma ty)
+
+with bidir_typed_chk :
+  forall {n : nat} (gamma : context n) (ct : cterm n) (ty : type) (const : constraints) (sigma : s_rules),
+  is_bidir_chk gamma ct ty const ->
+  sat_xi sigma const ->
+  is_typed (subst_ctx sigma gamma) (strip_chk ct) (subst_ty sigma ty).
+
+Proof.
+- intros n gamma st ty const sigma hb hs.
+  induction hb.
+  + simpl.
+    rewrite dist_subst_ty.
+    apply typed_abs.
+    rewrite <- cons_subst_ctx.
+    apply IHhb. apply hs.
+  + simpl.
+    apply bidir_typed_chk
+    with (const := const).
+    apply H. apply hs.
+- intros n gamma ct ty const sigma hb hs.
+  induction hb.
+  + simpl.
+    rewrite single_subst_ctx.
+    apply (typed_var (subst_ty sigma ty)).
+  + simpl.
+    rewrite app_subst_ctx.
+    apply typed_app
+    with (ty1 := (subst_ty sigma ty1)).
+    * rewrite <- dist_subst_ty.
+      apply IHhb.
+      apply appleft_sat_xi
+      with (const2 := const2).
+      apply hs.
+    * apply bidir_typed_syn
+      with (const := const2).
+      apply H.
+      apply appright_sat_xi
+      with (const1 := const1).
+      apply hs.
+  + simpl.
+    dependent destruction hs.
+    rewrite <- H0.
+    apply bidir_typed_syn
+    with (const := const).
+    apply H. apply hs.
+Qed.
+
+(* Unification *)
+
+(*
+Theorem bidir_subst_syn :
+  forall {n : nat} (gamma : context n) (st : sterm n) (ty : type) (const : constraints) (sigma1 sigma2 : s_rules),
+  is_bidir_syn gamma st ty const ->
+  sat_xi sigma1 const ->
+  Permutation sigma1 sigma2 ->
+  sat_xi sigma2 const
+
+with bidir_subst_chk :
+  forall {n : nat} (gamma : context n) (ct : cterm n) (ty : type) (const : constraints) (sigma1 sigma2 : s_rules),
+  is_bidir_chk gamma ct ty const ->
+  sat_xi sigma1 const ->
+  Permutation sigma1 sigma2 ->
+  sat_xi sigma2 const.
+Proof.
+- intros n gamma st ty const sigma1 sigma2 hb hs hp.
+  induction hb.
+  + apply IHhb. apply hs.
+  + apply bidir_subst_chk with
+    (n := n) (gamma := gamma)
+    (ct := ct) (ty := TVar a)
+    (sigma1 := sigma1).
+    apply H. apply hs. apply hp.
+- intros n gamma st ty const sigma1 sigma2 hb hs hp.
+  einduction hb.
+  + apply sat_nil.
+  + assert (sat_xi sigma1 const1).
+    apply appleft_sat_xi with (const2 := const2). apply hs.
+    assert (sat_xi sigma1 const2).
+    apply appright_sat_xi with (const1 := const1). apply hs.
+    assert (sat_xi sigma2 const1).
+    apply IHi. apply i. apply H0.
+    assert (sat_xi sigma2 const2).
+    apply bidir_subst_syn with
+    (n := m) (gamma := delta)
+    (st := st2) (ty := ty1)
+    (sigma1 := sigma1).
+    apply H. apply H1. apply hp.
+    apply app_sat_xi.
+    apply H2. apply H3.
+  + dependent destruction hs.
+    apply sat_cons.
+    apply bidir_subst_syn with
+    (n := n) (gamma := gamma)
+    (st := st) (ty := ty1)
+    (sigma1 := sigma).
+    apply H0. apply hs. apply hp.
+
+induction hp.
+* simpl. simpl in H. apply H.
+* simpl. simpl in H.
+*)
+
+Inductive build_subst : s_rules -> constraints -> Prop :=
+| build_nil : build_subst List.nil List.nil
+| build_consleft sigma const a ty :
+  build_subst sigma const ->
+  build_subst (sigma ++ (a, ty) :: List.nil)%list ((TVar a, ty) :: const)%list
+| build_consright sigma const b ty :
+  build_subst sigma const ->
+  build_subst (sigma ++ (b, ty) :: List.nil)%list ((ty, TVar b) :: const)%list
+| build_consimp sigma const tyA tyB tyC tyD :
+  build_subst sigma ((tyC, tyA) :: (tyB, tyD) :: const)%list ->
+  build_subst sigma ((TImp tyA tyC, TImp tyB tyD) :: const)%list.
+
+Inductive is_taut : constraints -> Prop :=
+| taut_nil : is_taut List.nil
+| taut_cons ty1 ty2 const :
+  is_taut const -> ty1 = ty2 ->
+  is_taut ((ty1, ty2) :: const)%list.
+
+Lemma nil_sat_taut : forall (const : constraints),
+  sat_xi List.nil const -> is_taut const.
+Proof.
+intros const h.
+dependent induction h.
+apply taut_nil.
+simpl in H.
+apply taut_cons.
+apply IHh.
+apply JMeq_refl.
+apply H.
+Qed.
+
+Lemma taut_sat_xi : forall (sigma : s_rules) (const : constraints),
+  is_taut const -> sat_xi sigma const.
+Proof.
+intros sigma const h.
+induction h.
+- apply sat_nil.
+- rewrite H.
+  apply sat_cons.
+  apply IHh.
+  reflexivity.
+Qed.
+
+Lemma subst_ty_last : forall (sigma : s_rules) (rul : s_rule) (ty : type),
+  subst_ty (sigma ++ rul :: Datatypes.nil)%list ty = 
+  subst1_ty rul (subst_ty sigma ty).
+Proof.
+intro sigma. induction sigma.
+- simpl. reflexivity.
+- intros rul ty. simpl.
+  apply IHsigma.
+Qed.
+
+Lemma skip_sat_xi : forall (sigma : s_rules) (rul : s_rule) (const : constraints),
+  sat_xi sigma const-> sat_xi (sigma ++ rul :: List.nil)%list const.
+Proof.
+intros.
+induction H.
+- apply sat_nil.
+- apply sat_cons.
+  apply IHsat_xi.
+  rewrite ? subst_ty_last.
+  rewrite H0.
+  reflexivity.
+Qed.
+
+(*
+Lemma build_sat : forall (sigma : s_rules) (const : constraints),
+  build_subst sigma const ->
+  sat_xi sigma const.
+Proof.
+intros sigma const h.
+induction h.
+- apply sat_nil.
+- apply sat_cons.
+  + apply skip_sat_xi. apply IHh.
+  + rewrite ? subst_ty_last.
+    simpl.
+
+
+  induction const.
+  + apply sat_nil.
+  + case_eq a0.
+    intros t1 t2 eq.
+    apply sat_cons.
+*)
+
+(*
+
 (*
 Consider: 
 unif_extra      only when !=Nil
@@ -171,6 +446,7 @@ Proof.
     apply unif_extra with (eq := (ty1, ty2)).
     apply hs.
 Qed.
+*)
 
 (* TODO: Principal Typing *)
 
